Remove WORLD outdated type (#14)
Squashed commit of the following:

commit a33d8680fb023a34eb19052ea3d9f38d3c024b1b
Author: June Rousseau <june.rousseau@cs.au.dk>
Date:   Wed Mar 5 14:33:26 2025 +0100

    Remove `WORLD : gmap CmptName CVIEW`

commit f32031daf4c23f38c32211f994168bd07dda5515
Author: June Rousseau <june.rousseau@cs.au.dk>
Date:   Wed Mar 5 11:06:49 2025 +0100

    Move lemma multiple update

commit ffb36e73d167c1998b2f967d9aefc32f53375dab
Author: June Rousseau <june.rousseau@cs.au.dk>
Date:   Wed Mar 5 10:43:05 2025 +0100

    Move lemmas about div and mod

theories/multiple_updates.v
@@ -18,118 +18,87 @@ Section std_updates.
 
   Notation STS := (leibnizO (STS_states * STS_rels)).
   Notation STS_STD := (leibnizO (STS_std_states Addr region_type)).
-  Notation CVIEW := (prodO STS_STD STS).
-  Notation WORLD := (gmapO CmptName CVIEW).
-  Implicit Types WC : CVIEW.
+  Notation WORLD := (prodO STS_STD STS).
   Implicit Types W : WORLD.
   Implicit Types C : CmptName.
 
-  Fixpoint std_update_multiple_cview WC l ρ :=
-    match l with
-    | [] => WC
-    | a :: l => std_update_cview (std_update_multiple_cview WC l ρ) a ρ
-    end.
-
-  Definition std_multiple_update W C l ρ :=
+  Fixpoint std_update_multiple W l ρ :=
     match l with
     | [] => W
-    | _ => (match W !! C with
-           | Some WC => <[C := std_update_multiple_cview WC l ρ]> W
-           | None => <[C := std_update_multiple_cview (∅,(∅,∅)) l ρ]> W
-           end)
+    | a :: l => std_update (std_update_multiple W l ρ) a ρ
     end.
 
-   Definition std_update_temp_multiple_cview WC l := std_update_multiple_cview WC l Temporary.
-   Definition std_update_temp_multiple W C l := std_multiple_update W C l Temporary.
+   Definition std_update_temp_multiple W l := std_update_multiple W l Temporary.
 
-   Lemma std_update_multiple_cview_loc_sta WC l ρ :
-     (std_update_multiple_cview WC l ρ).2.1 = WC.2.1.
+   Lemma std_update_multiple_loc_sta W l ρ :
+     (std_update_multiple W l ρ).2.1 = W.2.1.
    Proof.
      induction l; auto.
    Qed.
 
-   Lemma std_update_multiple_cview_loc_rel WC l ρ :
-     (std_update_multiple_cview WC l ρ).2.2 = WC.2.2.
+   Lemma std_update_multiple_loc_rel W l ρ :
+     (std_update_multiple W l ρ).2.2 = W.2.2.
    Proof.
      induction l; auto.
    Qed.
 
-   Lemma std_update_multiple_cview_loc WC l ρ :
-     (std_update_multiple_cview WC l ρ).2 = WC.2.
+   Lemma std_update_multiple_loc W l ρ :
+     (std_update_multiple W l ρ).2 = W.2.
    Proof.
      induction l; auto.
    Qed.
 
-   Lemma std_update_multiple_cview_proj_eq WC Wloc l ρ :
-     ((std_update_multiple_cview WC l ρ).1, Wloc) = std_update_multiple_cview (WC.1,Wloc) l ρ.
+   Lemma std_update_multiple_proj_eq W Wloc l ρ :
+     ((std_update_multiple W l ρ).1, Wloc) = std_update_multiple (W.1,Wloc) l ρ.
    Proof.
-     destruct WC as [Wsta Wloc']. simpl. induction l; auto.
+     destruct W as [Wsta Wloc']. simpl. induction l; auto.
      simpl. rewrite -IHl. auto.
    Qed.
 
-   Lemma std_update_multiple_cview_std_sta_eq WC Wloc l ρ :
-     (std_update_multiple_cview WC l ρ).1 = (std_update_multiple_cview (WC.1, Wloc) l ρ).1.
+   Lemma std_update_multiple_std_sta_eq W Wloc l ρ :
+     (std_update_multiple W l ρ).1 = (std_update_multiple (W.1, Wloc) l ρ).1.
    Proof.
-     destruct WC as [Wsta Wloc']. simpl. induction l; auto.
+     destruct W as [Wsta Wloc']. simpl. induction l; auto.
      simpl. rewrite -IHl. auto.
    Qed.
 
-   Lemma std_update_multiple_cview_swap_head WC l a1 a2 ρ :
-     std_update_multiple_cview WC (a1 :: a2 :: l) ρ = std_update_multiple_cview WC (a2 :: a1 :: l) ρ.
+   Lemma std_update_multiple_swap_head W l a1 a2 ρ :
+     std_update_multiple W (a1 :: a2 :: l) ρ = std_update_multiple W (a2 :: a1 :: l) ρ.
    Proof.
      induction l.
      - simpl. destruct (decide (a1 = a2)); subst.
        + done.
-       + rewrite /std_update_cview.
+       + rewrite /std_update.
          repeat rewrite (insert_commute _ a1 a2); auto.
      - destruct (decide (a1 = a2)); subst;[done|].
-       simpl. rewrite /std_update_cview.
+       simpl. rewrite /std_update.
        repeat rewrite (insert_commute _ a1 a2) ; auto.
    Qed.
 
-   Lemma std_update_multiple_cview_swap WC l1 a l2 ρ :
-     std_update_multiple_cview WC (l1 ++ a :: l2) ρ = std_update_multiple_cview WC (a :: l1 ++ l2) ρ.
+   Lemma std_update_multiple_swap W l1 a l2 ρ :
+     std_update_multiple W (l1 ++ a :: l2) ρ = std_update_multiple W (a :: l1 ++ l2) ρ.
    Proof.
      induction l1; auto.
-     rewrite app_comm_cons std_update_multiple_cview_swap_head /=.
+     rewrite app_comm_cons std_update_multiple_swap_head /=.
      f_equal;auto.
    Qed.
 
 
-   Lemma std_update_multiple_cview_permutation WC l1 l2 ρ :
+   Lemma std_update_multiple_permutation W l1 l2 ρ :
      l1 ≡ₚ l2 →
-     std_update_multiple_cview WC l1 ρ = std_update_multiple_cview WC l2 ρ.
+     std_update_multiple W l1 ρ = std_update_multiple W l2 ρ.
    Proof.
      intros Hperm.
      induction Hperm using Permutation_ind.
      - done.
      - simpl. rewrite IHHperm. done.
-     - apply (std_update_multiple_cview_swap_head WC l y x).
+     - apply (std_update_multiple_swap_head W l y x).
      - by rewrite IHHperm1 IHHperm2.
    Qed.
 
-   Lemma std_update_multiple_cview_permutation_C W C l1 l2 ρ :
-     l1 ≡ₚ l2 →
-     std_multiple_update W C l1 ρ = std_multiple_update W C l2 ρ.
-   Proof.
-     intros Hperm.
-     induction Hperm using Permutation_ind.
-     - done.
-     - rewrite /std_multiple_update.
-       destruct (W!!C); erewrite std_update_multiple_cview_permutation; eauto.
-     - rewrite /std_multiple_update.
-       destruct (W!!C); erewrite std_update_multiple_cview_permutation; eauto
-       ; apply Permutation_swap.
-     - by rewrite IHHperm1 -IHHperm2.
-   Qed.
-
-   Global Instance std_update_multiple_cview_Permutation WC ρ :
-     Proper (Permutation ==> eq) (λ l, std_update_multiple_cview WC l ρ).
-   Proof. intros y1 y2 Hperm. simpl. by apply std_update_multiple_cview_permutation. Defined.
-
-   Global Instance std_update_multiple_cview_Permutation_C W C ρ :
-     Proper (Permutation ==> eq) (λ l, std_multiple_update W C l ρ).
-   Proof. intros y1 y2 Hperm. by apply std_update_multiple_cview_permutation_C. Defined.
+   Global Instance std_update_multiple_Permutation W ρ :
+     Proper (Permutation ==> eq) (λ l, std_update_multiple W l ρ).
+   Proof. intros y1 y2 Hperm. simpl. by apply std_update_multiple_permutation. Defined.
 
    Lemma remove_dups_swap_head {A : Type} `{EqDecision A} (a1 a2 : A) (l : list A) :
      remove_dups (a1 :: a2 :: l) ≡ₚ remove_dups (a2 :: a1 :: l).
@@ -179,9 +148,9 @@ Section std_updates.
    (* --------------------------------------------------------------------------------------------------------- *)
 
    (* If an element is not in the update list, the state lookup is the same *)
-   Lemma std_sta_update_multiple_lookup_same_i WC l ρ i :
-     i ∉ l -> (std_cview (std_update_multiple_cview WC l ρ)) !! i =
-             (std_cview WC) !! i.
+   Lemma std_sta_update_multiple_lookup_same_i W l ρ i :
+     i ∉ l -> (std (std_update_multiple W l ρ)) !! i =
+             (std W) !! i.
    Proof.
      intros Hnin.
      induction l; auto.
@@ -192,8 +161,8 @@ Section std_updates.
    (* ------------------------------------------------------------ *)
 
    (* If an element is in the update list, the state lookup corresponds to the update value *)
-   Lemma std_sta_update_multiple_lookup_in_i WC l ρ i :
-     i ∈ l -> (std_cview (std_update_multiple_cview WC l ρ)) !! i = Some ρ.
+   Lemma std_sta_update_multiple_lookup_in_i W l ρ i :
+     i ∈ l -> (std (std_update_multiple W l ρ)) !! i = Some ρ.
    Proof.
      intros Hnin.
      induction l; auto; first inversion Hnin.
@@ -206,8 +175,8 @@ Section std_updates.
    (* ------------------------------------------------------------ *)
 
    (* if W at a is_Some, the the updated W at a is_Some *)
-   Lemma std_sta_update_multiple_is_Some WC l ρ i :
-     is_Some (std_cview WC !! i) -> is_Some (std_cview (std_update_multiple_cview WC l ρ) !! i).
+   Lemma std_sta_update_multiple_is_Some W l ρ i :
+     is_Some (std W !! i) -> is_Some (std (std_update_multiple W l ρ) !! i).
    Proof.
      intros Hsome.
      destruct (decide (i ∈ l)).
@@ -218,17 +187,17 @@ Section std_updates.
    (* ------------------------------------------------------------ *)
 
    (* domains *)
-   Lemma std_update_multiple_cview_not_in_sta_i WC l ρ i :
-     i ∉ l → i ∈ dom (std_cview WC) ↔
-               i ∈ dom (std_cview (std_update_multiple_cview WC l ρ)).
+   Lemma std_update_multiple_not_in_sta_i W l ρ i :
+     i ∉ l → i ∈ dom (std W) ↔
+               i ∈ dom (std (std_update_multiple W l ρ)).
    Proof.
      intros Hnin. induction l; auto.
      apply not_elem_of_cons in Hnin as [Hneq Hnin].
      rewrite /= dom_insert. set_solver.
    Qed.
-   Lemma std_update_multiple_cview_in_sta_i WC (l: list Addr) ρ i :
-     Forall (λ (a:Addr), is_Some (std_cview WC !! a)) l →
-     i ∈ dom (std_cview WC) ↔ i ∈ dom (std_cview (std_update_multiple_cview WC l ρ)).
+   Lemma std_update_multiple_in_sta_i W (l: list Addr) ρ i :
+     Forall (λ (a:Addr), is_Some (std W !! a)) l →
+     i ∈ dom (std W) ↔ i ∈ dom (std (std_update_multiple W l ρ)).
    Proof.
      intros Hl.
      induction l; auto.
@@ -237,95 +206,56 @@ Section std_updates.
      rewrite elem_of_union elem_of_singleton. intros [-> | Hi]; [| set_solver].
      rewrite elem_of_dom //.
    Qed.
-   Lemma std_update_multiple_cview_not_in_sta WC l ρ (a : Addr) :
-     a ∉ l → a ∈ dom (std_cview WC) ↔
-             a ∈ dom (std_cview (std_update_multiple_cview WC l ρ)).
+   Lemma std_update_multiple_not_in_sta W l ρ (a : Addr) :
+     a ∉ l → a ∈ dom (std W) ↔
+             a ∈ dom (std (std_update_multiple W l ρ)).
    Proof.
      intros Hnin.
-     apply std_update_multiple_cview_not_in_sta_i.
+     apply std_update_multiple_not_in_sta_i.
      intros Hcontr. contradiction.
    Qed.
 
    (* ---------------------------------------------------------------------------- *)
    (* Some helper lemmas for various lemmas about using multiple updates in region *)
 
-   Lemma related_sts_pub_update_multiple_cview WC l ρ :
-     Forall (λ a, a ∉ dom (std_cview WC)) l →
-     related_sts_pub_cview WC (std_update_multiple_cview WC l ρ).
+   Lemma related_sts_pub_update_multiple W l ρ :
+     Forall (λ a, a ∉ dom (std W)) l →
+     related_sts_pub_world W (std_update_multiple W l ρ).
    Proof.
      intros Hforall. induction l.
-     - apply related_sts_pub_refl_cview.
+     - apply related_sts_pub_refl_world.
      - simpl.
        apply list.Forall_cons in Hforall as [ Ha_std Hforall].
-       eapply related_sts_pub_trans_cview;[apply IHl; auto|].
+       eapply related_sts_pub_trans_world;[apply IHl; auto|].
        destruct (decide (a ∈ l)).
-       { rewrite (_: <s[a:=ρ]s>(std_update_multiple_cview WC l ρ) = std_update_multiple_cview WC l ρ) /=.
-         by apply related_sts_pub_refl_cview.
-         rewrite /std_update_cview insert_id /=. by destruct (std_update_multiple_cview WC l ρ).
+       { rewrite (_: <s[a:=ρ]s>(std_update_multiple W l ρ) = std_update_multiple W l ρ) /=.
+         by apply related_sts_pub_refl_world.
+         rewrite /std_update insert_id /=. by destruct (std_update_multiple W l ρ).
          by apply std_sta_update_multiple_lookup_in_i. }
-       apply related_sts_pub_cview_fresh; auto.
-       intros Hcontr. apply std_update_multiple_cview_not_in_sta in Hcontr; auto.
+       apply related_sts_pub_world_fresh; auto.
+       intros Hcontr. apply std_update_multiple_not_in_sta in Hcontr; auto.
    Qed.
 
-   Lemma related_sts_pub_update_multiple W C l ρ :
-     Forall (λ a, a ∉ dom (std W C)) l →
-     related_sts_pub_world W (std_multiple_update W C l ρ) C.
-   Proof.
-     intros Hforall.
-     rewrite /std in Hforall.
-     rewrite /std_multiple_update.
-     destruct l as [|a l]; first apply related_sts_pub_refl_world.
-     destruct (W!!C) as [WC|] eqn:HWC.
-     - split.
-       + rewrite dom_insert_L ; set_solver.
-       + intros ? WC' ? HWC' ; rewrite lookup_insert in HWC' ; simplify_eq.
-         by apply related_sts_pub_update_multiple_cview.
-     - split.
-       + rewrite dom_insert_L ; set_solver.
-       + intros ? WC' ? HWC' ; rewrite lookup_insert in HWC' ; simplify_eq.
-   Qed.
-
-   Lemma std_update_multiple_cview_lookup_cview WC l ρ k y :
+   Lemma std_update_multiple_lookup W l ρ k y :
      l !! k = Some y ->
-     std_cview (std_update_multiple_cview WC l ρ) !! y = Some ρ.
+     std (std_update_multiple W l ρ) !! y = Some ρ.
    Proof.
      intros Helem.
      apply elem_of_list_lookup_2 in Helem.
      apply elem_of_list_split in Helem as [l1 [l2 Heq] ].
-     rewrite Heq std_update_multiple_cview_swap /= /std_update_cview.
-     rewrite /std_cview /=. rewrite lookup_insert. auto.
-   Qed.
-
-   Lemma std_update_multiple_cview_lookup W C l ρ k y :
-     l !! k = Some y ->
-     is_Some (W!!C) ->
-     std (std_multiple_update W C l ρ) C !! y = Some ρ.
-   Proof.
-     intros Helem [WC HWC].
-     rewrite /std /std_multiple_update HWC.
-     destruct l ; first done.
-     rewrite lookup_insert. eapply std_update_multiple_cview_lookup_cview; eauto.
-   Qed.
-
-   Lemma std_update_temp_multiple_lookup W C l k y :
-     l !! k = Some y →
-     is_Some (W!!C) ->
-     region_state_pwl (std_update_temp_multiple W C l) C y.
-   Proof.
-     intros Helem HWC.
-     rewrite /std_update_temp_multiple.
-     eapply std_update_multiple_cview_lookup; eauto.
+     rewrite Heq std_update_multiple_swap /= /std_update.
+     rewrite /std /=. rewrite lookup_insert. auto.
    Qed.
 
 
    (* Multiple updates does not change dom, as long as the updated elements are a subset of original dom *)
-   Lemma std_update_multiple_cview_dom_equal WC l ρ :
-     (∀ i : Addr, i ∈ l → i ∈ dom (std_cview WC)) ->
-     dom (std_cview WC) = dom (std_cview (std_update_multiple_cview WC l ρ)).
+   Lemma std_update_multiple_dom_equal W l ρ :
+     (∀ i : Addr, i ∈ l → i ∈ dom (std W)) ->
+     dom (std W) = dom (std (std_update_multiple W l ρ)).
    Proof.
      intros Hsub.
      induction l; auto.
-     rewrite /= /std_update_cview.
+     rewrite /= /std_update.
      rewrite dom_insert_L.
      assert (a ∈ a :: l) as Hin.
      { apply elem_of_cons. by left. }
@@ -335,121 +265,51 @@ Section std_updates.
    Qed.
 
    (* In general, the domain is a subset of the updated domain *)
-   Lemma std_update_multiple_cview_sta_dom_subseteq WC l ρ :
-     dom (std_cview WC) ⊆ dom (std_cview (std_update_multiple_cview WC l ρ)).
+   Lemma std_update_multiple_sta_dom_subseteq W l ρ :
+     dom (std W) ⊆ dom (std (std_update_multiple W l ρ)).
    Proof.
      apply elem_of_subseteq. intros x Hx.
      destruct (decide (x ∈ l)).
      - rewrite elem_of_dom. exists ρ.
        apply std_sta_update_multiple_lookup_in_i; auto.
-     - apply std_update_multiple_cview_not_in_sta_i; auto.
+     - apply std_update_multiple_not_in_sta_i; auto.
    Qed.
 
-   Lemma std_update_multiple_cview_std_sta_dom_monotone_cview WC WC' l ρ :
-     dom (std_cview WC) ⊆ dom (std_cview WC') ->
-     dom (std_cview (std_update_multiple_cview WC l ρ)) ⊆ dom (std_cview (std_update_multiple_cview WC' l ρ)).
+   Lemma std_update_multiple_std_sta_dom_monotone W W' l ρ :
+     dom (std W) ⊆ dom (std W') ->
+     dom (std (std_update_multiple W l ρ)) ⊆ dom (std (std_update_multiple W' l ρ)).
    Proof.
      induction l;auto.
      simpl. repeat rewrite dom_insert_L. set_solver.
    Qed.
 
-   Lemma std_update_multiple_cview_std_sta_dom_monotone W W' C l ρ :
-     dom W ⊆ dom W' ->
-     dom (std W C) ⊆ dom (std W' C) ->
-     dom (std (std_multiple_update W C l ρ) C) ⊆ dom (std (std_multiple_update W' C l ρ) C).
-   Proof.
-     rewrite /std /std_multiple_update.
-     intros Hdom_W Hdom.
-     destruct l ; first done.
-     destruct (W !! C) as [WC|] eqn:HWC.
-     - rewrite lookup_insert.
-       assert (is_Some (W' !! C)) as [WC' HWC'].
-       {
-         apply (elem_of_dom_2 W) in HWC.
-         specialize (Hdom_W _ HWC).
-         by eapply (elem_of_dom W').
-       }
-       rewrite HWC' lookup_insert.
-       rewrite HWC' in Hdom.
-       by eapply std_update_multiple_cview_std_sta_dom_monotone_cview.
-     - rewrite lookup_insert.
-       destruct (W'!!C) as [WC'|] eqn:HWC'; rewrite lookup_insert; auto.
-       by eapply std_update_multiple_cview_std_sta_dom_monotone_cview.
-   Qed.
-
-   Lemma std_update_multiple_related_monotone_cview WC WC' l ρ :
-     related_sts_pub_cview WC WC' ->
-     related_sts_pub_cview (std_update_multiple_cview WC l ρ) (std_update_multiple_cview WC' l ρ).
+   Lemma std_update_multiple_related_monotone W W' l ρ :
+     related_sts_pub_world W W' ->
+     related_sts_pub_world (std_update_multiple W l ρ) (std_update_multiple W' l ρ).
    Proof.
      intros Hrelated.
-     destruct WC as [ Wstd_sta [Wloc_sta Wloc_rel] ].
-     destruct WC' as [ Wstd_sta' [Wloc_sta' Wloc_rel'] ].
+     destruct W as [ Wstd_sta [Wloc_sta Wloc_rel] ].
+     destruct W' as [ Wstd_sta' [Wloc_sta' Wloc_rel'] ].
      destruct Hrelated as [ [Hstd_dom1 Hstd_related ] Hloc_related].
      simpl in *.
-     split;[clear Hloc_related|by repeat rewrite std_update_multiple_cview_loc_rel std_update_multiple_cview_loc_sta].
+     split;[clear Hloc_related|by repeat rewrite std_update_multiple_loc_rel std_update_multiple_loc_sta].
      split.
-     - apply std_update_multiple_cview_std_sta_dom_monotone_cview. auto.
+     - apply std_update_multiple_std_sta_dom_monotone. auto.
      - intros i x y Hx Hy.
        destruct (decide (i ∈ l)).
        + rewrite std_sta_update_multiple_lookup_in_i in Hx;auto.
          rewrite std_sta_update_multiple_lookup_in_i in Hy;auto.
          inversion Hx; inversion Hy; subst. left.
-       + rewrite std_sta_update_multiple_lookup_same_i /std_cview /= in Hx;auto.
-         rewrite std_sta_update_multiple_lookup_same_i /std_cview /= in Hy;auto.
+       + rewrite std_sta_update_multiple_lookup_same_i /std /= in Hx;auto.
+         rewrite std_sta_update_multiple_lookup_same_i /std /= in Hy;auto.
          apply Hstd_related with i; auto.
    Qed.
 
-   Lemma std_update_multiple_dom_monotone W W' C l ρ :
-     dom W ⊆ dom W' ->
-     dom (std_multiple_update W C l ρ) ⊆ dom (std_multiple_update W' C l ρ).
-    Proof.
-      intros Hdom.
-      rewrite /std_multiple_update.
-      destruct l ; first done.
-      destruct (W !! C) as [WC|] eqn:HWC; eauto.
-      - destruct (W' !! C) as [WC'|] eqn:HWC'; eauto.
-        + rewrite !dom_insert_L; set_solver.
-        + eapply (elem_of_dom_2 W) in HWC.
-          specialize (Hdom _ HWC).
-          by eapply (not_elem_of_dom W') in HWC'.
-      - destruct (W' !! C) as [WC'|] eqn:HWC'; eauto.
-        + rewrite !dom_insert_L; set_solver.
-        + rewrite !dom_insert_L; set_solver.
-    Qed.
-
-   Lemma std_update_multiple_related_monotone W W' C l ρ :
-     related_sts_pub_world W W' C ->
-     related_sts_pub_world (std_multiple_update W C l ρ) (std_multiple_update W' C l ρ) C.
-   Proof.
-     intros [Hdom Hrelated].
-     split.
-     - by apply std_update_multiple_dom_monotone.
-     - rewrite /std_multiple_update.
-       destruct l ; first done.
-       intros WC_upd WC_upd' HWC_upd HWC_upd'.
-       destruct (W!!C) as [WC|] eqn:HWC.
-       + destruct (W'!!C) as [WC'|] eqn:HWC' ; cycle 1.
-         { eapply (elem_of_dom_2 W) in HWC.
-           specialize (Hdom _ HWC).
-           by eapply (not_elem_of_dom W') in HWC'.
-         }
-         rewrite lookup_insert in HWC_upd; rewrite lookup_insert in HWC_upd'; simplify_eq.
-         apply std_update_multiple_related_monotone_cview.
-         by apply Hrelated.
-       + destruct (W'!!C) as [WC'|] eqn:HWC'; simplify_eq.
-         all: rewrite lookup_insert in HWC_upd.
-         all: rewrite lookup_insert in HWC_upd'.
-         all: simplify_eq.
-         * apply std_update_multiple_related_monotone_cview.
-           apply related_sts_pub_empty_cview.
-         * by apply std_update_multiple_related_monotone_cview.
-   Qed.
-
    (* lemmas for updating a repetition of top *)
-   Lemma std_update_multiple_cview_dom_top_sta WC n ρ a :
+   Lemma std_update_multiple_dom_top_sta W n ρ a :
      a ≠ addr_reg.top ->
-     a ∉ dom (std_cview WC) →
-     a ∉ dom (std_cview (std_update_multiple_cview WC (repeat addr_reg.top n) ρ)).
+     a ∉ dom (std W) →
+     a ∉ dom (std (std_update_multiple W (repeat addr_reg.top n) ρ)).
    Proof.
      intros Hne Hnin.
      induction n; auto.
@@ -460,10 +320,10 @@ Section std_updates.
      + apply IHn.
    Qed.
 
-   Lemma std_update_multiple_cview_dom_sta_i WC n ρ a i :
+   Lemma std_update_multiple_dom_sta_i W n ρ a i :
      a ≠ addr_reg.top → (i > 0)%Z →
-     a ∉ dom (std_cview WC) →
-     a ∉ dom (std_cview (std_update_multiple_cview WC (finz.seq ((a ^+ i)%a) n) ρ)).
+     a ∉ dom (std W) →
+     a ∉ dom (std (std_update_multiple W (finz.seq ((a ^+ i)%a) n) ρ)).
    Proof.
      intros Hneq Hgt.
      destruct (a + i)%a eqn:Hsome.
@@ -482,9 +342,9 @@ Section std_updates.
          ++ replace ((a ^+ j) ^+ 1)%a with (a ^+ (j+1))%a by solve_addr.
             apply incr_addr_one_none in Ha2.
             replace (a ^+ (j + 1))%a with (finz.largest 0%a) by solve_addr.
-            rewrite finz_seq_top. apply std_update_multiple_cview_dom_top_sta; auto.
+            rewrite finz_seq_top. apply std_update_multiple_dom_top_sta; auto.
      - replace (a ^+ i)%a with (finz.largest 0%a) by solve_addr.
-       rewrite finz_seq_top. apply std_update_multiple_cview_dom_top_sta; auto.
+       rewrite finz_seq_top. apply std_update_multiple_dom_top_sta; auto.
    Qed.
 
    Lemma incr_addr_is_Some_weak a n :
@@ -494,10 +354,10 @@ Section std_updates.
      solve_addr.
    Qed.
 
-   Lemma std_sta_update_multiple_insert WC (a b a' l : Addr) ρ i :
+   Lemma std_sta_update_multiple_insert W (a b a' l : Addr) ρ i :
      (a' < a)%a →
-     std_cview (std_update_multiple_cview (std_update_cview WC a' i) (finz.seq_between a b) ρ) !! l =
-     std_cview (std_update_cview (std_update_multiple_cview WC (finz.seq_between a b) ρ) a' i) !! l.
+     std (std_update_multiple (std_update W a' i) (finz.seq_between a b) ρ) !! l =
+     std (std_update (std_update_multiple W (finz.seq_between a b) ρ) a' i) !! l.
    Proof.
      intros Hlt.
      destruct (decide (l ∈ finz.seq_between a b)) as [Hin|Hin].
@@ -507,25 +367,25 @@ Section std_updates.
          solve_addr.
        }
        apply elem_of_list_lookup in Hin as [n Hsome].
-       assert (std_cview (std_update_multiple_cview WC (finz.seq_between a b) ρ) !! l = Some ρ) as Hpwl.
-       { apply std_update_multiple_cview_lookup_cview with n; auto. }
-       assert (std_cview (std_update_multiple_cview (std_update_cview WC a' i) (finz.seq_between a b) ρ) !! l = Some ρ) as Hpwl'.
-       { apply std_update_multiple_cview_lookup_cview with n; auto. }
+       assert (std (std_update_multiple W (finz.seq_between a b) ρ) !! l = Some ρ) as Hpwl.
+       { apply std_update_multiple_lookup with n; auto. }
+       assert (std (std_update_multiple (std_update W a' i) (finz.seq_between a b) ρ) !! l = Some ρ) as Hpwl'.
+       { apply std_update_multiple_lookup with n; auto. }
        rewrite -Hpwl in Hpwl'. rewrite Hpwl'.
        rewrite lookup_insert_ne; auto.
      - rewrite std_sta_update_multiple_lookup_same_i; auto.
        destruct (decide ( a' =  l)).
-       + rewrite /std_update_cview /std_cview /= e. do 2 rewrite lookup_insert. done.
-       + rewrite /std_update_cview /std_cview /=. rewrite lookup_insert_ne;auto. rewrite lookup_insert_ne; auto.
+       + rewrite /std_update /std /= e. do 2 rewrite lookup_insert. done.
+       + rewrite /std_update /std /=. rewrite lookup_insert_ne;auto. rewrite lookup_insert_ne; auto.
          rewrite std_sta_update_multiple_lookup_same_i; auto.
    Qed.
 
-   Lemma std_update_multiple_cview_dom_insert WC (a b a' : Addr) i :
+   Lemma std_update_multiple_dom_insert W (a b a' : Addr) i :
      (a' < a)%a →
      Forall (λ a : Addr,
-                   (a ∉ dom (std_cview WC))) (finz.seq_between a b) →
+                   (a ∉ dom (std W))) (finz.seq_between a b) →
      Forall (λ a : Addr,
-                   (a ∉ dom (<[ a' := i]> WC.1))) (finz.seq_between a b).
+                   (a ∉ dom (<[ a' := i]> W.1))) (finz.seq_between a b).
    Proof.
      intros Hlt.
      do 2 (rewrite list.Forall_forall). intros Hforall.
@@ -543,14 +403,14 @@ Section std_updates.
 
    (* commuting updates and revoke *)
 
-   Lemma std_update_multiple_cview_revoke_commute_cview WC (l: list Addr) ρ :
+   Lemma std_update_multiple_revoke_commute W (l: list Addr) ρ :
      ρ ≠ Temporary → ρ ≠ Temporary →
-     std_update_multiple_cview (revoke_cview WC) l ρ = revoke_cview (std_update_multiple_cview WC l ρ).
+     std_update_multiple (revoke W) l ρ = revoke (std_update_multiple W l ρ).
    Proof.
      intros Hne Hne'.
      induction l; auto; simpl.
      rewrite IHl.
-     rewrite /std_update_cview /revoke_cview /loc /std_cview /=. repeat f_equiv.
+     rewrite /std_update /revoke /loc /std /=. repeat f_equiv.
      eapply (map_leibniz (M:=gmap Addr) (A:=region_type)). intros i. eapply leibniz_equiv_iff.
      destruct (decide (a = i)).
      - subst. rewrite lookup_insert revoke_monotone_lookup_same;rewrite lookup_insert; auto.
@@ -561,80 +421,27 @@ Section std_updates.
        apply option_leibniz.
    Qed.
 
-   Lemma std_update_multiple_cview_revoke_commute W C (l: list Addr) ρ :
-     ρ ≠ Temporary → ρ ≠ Temporary →
-     std_multiple_update (revoke W C) C l ρ = revoke (std_multiple_update W C l ρ) C.
-   Proof.
-     intros Hne Hne'.
-     rewrite /std_multiple_update /revoke.
-     destruct l ; first done.
-     destruct (W!!C) as [WC|] eqn:HWC; [|rewrite HWC]
-     ; rewrite !lookup_insert !insert_insert.
-     - by rewrite std_update_multiple_cview_revoke_commute_cview.
-     - rewrite -std_update_multiple_cview_revoke_commute_cview;auto.
-   Qed.
-   (* std_update_multiple_cview and app *)
-
-   Lemma std_update_multiple_cview_app WC (l1 l2 : list Addr) ρ :
-     std_update_multiple_cview WC (l1 ++ l2) ρ = std_update_multiple_cview (std_update_multiple_cview WC l1 ρ) l2 ρ.
+   Lemma std_update_multiple_app W (l1 l2 : list Addr) ρ :
+     std_update_multiple W (l1 ++ l2) ρ = std_update_multiple (std_update_multiple W l1 ρ) l2 ρ.
    Proof.
      induction l2; auto.
      - by rewrite app_nil_r /=.
-     - rewrite std_update_multiple_cview_swap /=. f_equal. auto.
+     - rewrite std_update_multiple_swap /=. f_equal. auto.
    Qed.
 
-   Lemma std_update_multiple_cview_app_commute WC (l1 l2 : list Addr) ρ :
-     std_update_multiple_cview WC (l1 ++ l2) ρ = std_update_multiple_cview WC (l2 ++ l1) ρ.
+   Lemma std_update_multiple_app_commute W (l1 l2 : list Addr) ρ :
+     std_update_multiple W (l1 ++ l2) ρ = std_update_multiple W (l2 ++ l1) ρ.
    Proof.
      induction l2.
      - by rewrite app_nil_r /=.
-     - rewrite std_update_multiple_cview_swap /=. by rewrite IHl2.
+     - rewrite std_update_multiple_swap /=. by rewrite IHl2.
    Qed.
 
-   Lemma revoke_condition_std_multiple_updates W C l ρ :
-     revoke_condition W C
-     → ρ ≠ Temporary
-     → revoke_condition (std_multiple_update W C l ρ) C.
-   Proof.
-     induction l as [|a l IHl].
-     - intros Hrev Hne.
-       rewrite /std_multiple_update; done.
-     - simpl. intros Hrev Hne a'.
-       destruct (W!!C) as [WC|] eqn:HWC; cycle 1.
-       { destruct (decide (a = a')); simplify_map_eq.
-         + rewrite /std lookup_insert.
-           rewrite lookup_insert. congruence.
-         + apply IHl in Hrev; auto.
-           rewrite /revoke_condition in Hrev.
-           (* rewrite /std /std_multiple_update HWC in Hrev. *)
-           rewrite /std lookup_insert.
-           rewrite lookup_insert_ne; auto.
-           specialize (Hrev a').
-           destruct l; first done.
-           by rewrite /std /std_multiple_update HWC lookup_insert in Hrev.
-       }
-       rewrite /std lookup_insert.
-       destruct (decide (a = a')).
-       + simpl. destruct WC as [Wstd Wloc].
-         rewrite (std_update_multiple_cview_std_sta_eq _ Wloc). subst. rewrite lookup_insert.
-         congruence.
-       + simpl. destruct WC as [Wstd Wloc].
-         rewrite (std_update_multiple_cview_std_sta_eq _ Wloc). rewrite lookup_insert_ne//.
-         apply IHl in Hrev;auto.
-         cbn.
-         rewrite /revoke_condition in Hrev.
-         destruct l.
-         * rewrite /std /std_multiple_update HWC in Hrev.
-           done.
-         * rewrite /std /std_multiple_update HWC lookup_insert in Hrev.
-           done.
-   Qed.
-
-   Lemma std_update_multiple_cview_overlap WC l ρ1 ρ2 :
-     std_update_multiple_cview (std_update_multiple_cview WC l ρ1) l ρ2 = std_update_multiple_cview WC l ρ2.
+   Lemma std_update_multiple_overlap W l ρ1 ρ2 :
+     std_update_multiple (std_update_multiple W l ρ1) l ρ2 = std_update_multiple W l ρ2.
    Proof.
      induction l;auto.
-     simpl. destruct WC as [Wstd Wloc]. rewrite /std_update_cview /=. rewrite !std_update_multiple_cview_loc /=. f_equiv.
+     simpl. destruct W as [Wstd Wloc]. rewrite /std_update /=. rewrite !std_update_multiple_loc /=. f_equiv.
      apply map_eq'. intros k v.
      destruct (decide (a = k)).
      + subst. rewrite !lookup_insert. auto.
@@ -644,50 +451,49 @@ Section std_updates.
          rewrite lookup_insert_ne//. rewrite !std_sta_update_multiple_lookup_same_i// /=.
    Qed.
 
-   Lemma std_update_multiple_cview_insert_commute WC a (l: list Addr) ρ ρ' :
+   Lemma std_update_multiple_insert_commute W a (l: list Addr) ρ ρ' :
      a ∉ l →
-     std_update_multiple_cview (<s[a:=ρ']s> WC) l ρ = <s[a:=ρ']s> (std_update_multiple_cview WC l ρ).
+     std_update_multiple (<s[a:=ρ']s> W) l ρ = <s[a:=ρ']s> (std_update_multiple W l ρ).
    Proof.
      intros Hne.
      induction l; auto; simpl.
      apply not_elem_of_cons in Hne as [Hne Hnin].
      rewrite IHl;auto.
-     rewrite /std_update_cview /revoke_cview /loc /std_cview /=. rewrite insert_commute;auto.
+     rewrite /std_update /revoke /loc /std /=. rewrite insert_commute;auto.
    Qed.
 
-   Lemma related_sts_pub_update_multiple_perm_cview WC l :
-     Forall (λ k, std_cview WC !! k = Some Revoked) l →
-     related_sts_pub_cview WC (std_update_multiple_cview WC l Permanent).
+   Lemma related_sts_pub_update_multiple_perm W l :
+     Forall (λ k, std W !! k = Some Revoked) l →
+     related_sts_pub_world W (std_update_multiple W l Permanent).
    Proof.
      intros Hforall. induction l.
-     - apply related_sts_pub_refl_cview.
+     - apply related_sts_pub_refl_world.
      - simpl.
        apply list.Forall_cons in Hforall as [ Ha_std Hforall].
-       eapply related_sts_pub_trans_cview;[apply IHl; auto|].
+       eapply related_sts_pub_trans_world;[apply IHl; auto|].
        destruct (decide (a ∈ l)).
-       { rewrite (_: <s[a:=Permanent]s>(std_update_multiple_cview WC l Permanent) = std_update_multiple_cview WC l Permanent) /=.
-         by apply related_sts_pub_refl_cview.
-         rewrite /std_update_cview insert_id /=. by destruct (std_update_multiple_cview WC l Permanent).
+       { rewrite (_: <s[a:=Permanent]s>(std_update_multiple W l Permanent) = std_update_multiple W l Permanent) /=.
+         by apply related_sts_pub_refl_world.
+         rewrite /std_update insert_id /=. by destruct (std_update_multiple W l Permanent).
          by apply std_sta_update_multiple_lookup_in_i. }
-       destruct WC as [Hstd_cview Hloc].
-       apply related_sts_pub_world_revoked_permanent_cview in Ha_std.
-       eapply related_sts_pub_trans_cview;[apply std_update_multiple_related_monotone_cview,Ha_std|].
-       rewrite std_update_multiple_cview_insert_commute //. apply related_sts_pub_refl_cview.
+       destruct W as [Hstd Hloc].
+       apply related_sts_pub_world_revoked_permanent in Ha_std.
+       eapply related_sts_pub_trans_world;[apply std_update_multiple_related_monotone,Ha_std|].
+       rewrite std_update_multiple_insert_commute //. apply related_sts_pub_refl_world.
    Qed.
 
-   Lemma related_sts_pub_update_multiple_perm W C l :
-     Forall (λ k, std W C !! k = Some Revoked) l →
-     related_sts_pub_world W (std_multiple_update W C l Permanent) C.
-   Proof.
-     intros Hforall.
-     destruct l; first apply related_sts_pub_refl_world.
-     split.
-     - rewrite /std_multiple_update.
-       destruct (W!!C) ; rewrite dom_insert_L; set_solver.
-     - intros WC WC' HWC HWC'.
-       rewrite /std_multiple_update HWC lookup_insert in HWC'; simplify_eq.
-       rewrite /std HWC in Hforall.
-       by apply related_sts_pub_update_multiple_perm_cview.
-   Qed.
+  Lemma elem_of_dom_std_multiple_update (W : WORLD) (a : Addr) (l : list Addr)
+    (ρ: region_type) :
+    a ∈ (dom (std (std_update_multiple W l ρ))) ->
+    a ∈ l \/ a ∈ (dom (std W)).
+  Proof.
+    induction l as [|a' l] ; intros Ha; first naive_solver.
+    destruct (decide (a = a')) as [|Hna]; simplify_eq; first (left; set_solver).
+    destruct (decide (a ∈ l)) as [|Hnl]; first (left; set_solver).
+    right.
+    rewrite /= /std dom_insert_L elem_of_union in Ha.
+    destruct Ha as [Ha|Ha] ; first ( rewrite elem_of_singleton in Ha ; set_solver ).
+    apply IHl in Ha. destruct Ha; done.
+  Qed.
 
 End std_updates.
