theories/ftlr/Lea.v
@@ -9,17 +9,15 @@ From cap_machine.proofmode Require Import map_simpl register_tactics.
 Section fundamental.
   Context
     {Σ:gFunctors}
-      {ceriseg:ceriseG Σ} {sealsg: sealStoreG Σ}
-      {Cname : CmptNameG}
-      {stsg : STSG Addr region_type Σ} {heapg : heapGS Σ}
-      {nainv: logrel_na_invs Σ}
-      `{MP: MachineParameters}.
+    {ceriseg:ceriseG Σ} {sealsg: sealStoreG Σ}
+    {Cname : CmptNameG}
+    {stsg : STSG Addr region_type Σ} {heapg : heapGS Σ}
+    {nainv: logrel_na_invs Σ}
+    `{MP: MachineParameters}.
 
   Notation STS := (leibnizO (STS_states * STS_rels)).
   Notation STS_STD := (leibnizO (STS_std_states Addr region_type)).
-  Notation CVIEW := (prodO STS_STD STS).
-  Notation WORLD := (gmapO CmptName CVIEW).
-  Implicit Types WC : CVIEW.
+  Notation WORLD := (prodO STS_STD STS).
   Implicit Types W : WORLD.
   Implicit Types C : CmptName.
 
