theories/ftlr/Store.v
@@ -19,9 +19,7 @@ Section fundamental.
 
   Notation STS := (leibnizO (STS_states * STS_rels)).
   Notation STS_STD := (leibnizO (STS_std_states Addr region_type)).
-  Notation CVIEW := (prodO STS_STD STS).
-  Notation WORLD := (gmapO CmptName CVIEW).
-  Implicit Types WC : CVIEW.
+  Notation WORLD := (prodO STS_STD STS).
   Implicit Types W : WORLD.
   Implicit Types C : CmptName.
 
@@ -41,7 +39,7 @@ Section fundamental.
      PermFlowsTo p p'
     -> word_of_argument r r2 = Some storev
     → reg_allows_store r r1 p g b e a storev
-    → std W C !! a = Some ρ
+    → std W !! a = Some ρ
     → interp W C (WCap p g b e a)
     -∗ monotonicity_guarantees_region C interpC p' storev ρ.
   Proof.
@@ -86,7 +84,7 @@ Section fundamental.
     (v : Word) (P : D) (has_later : bool): iProp Σ :=
     (∃ ρ,
         sts_state_std C l ρ
-        ∗ ⌜std W C !! l = Some ρ⌝
+        ∗ ⌜std W !! l = Some ρ⌝
         ∗ ⌜ρ ≠ Revoked⌝
         ∗ ⌜(∀ g, ρ ≠ Frozen g)⌝
         ∗ open_region_many W C (l :: ls)
@@ -278,7 +276,7 @@ Section fundamental.
     (W : WORLD) (C : CmptName)
     (p : Perm) (w : Word) (P : D)
     (a : Addr) (ρ : region_type) :
-    std W C !! a = Some ρ
+    std W !! a = Some ρ
     -> ρ ≠ Revoked
     -> (∀ m, ρ ≠ Frozen m)
     -> canStore p w = true
@@ -299,7 +297,7 @@ Section fundamental.
      (mem0 : Mem) (oldv storev : Word) (ρ : region_type) (P:D):
      word_of_argument (<[PC:= WCap pc_p pc_g pc_b pc_e pc_a]> regs) r2 = Some storev
     → reg_allows_store (<[PC:= WCap pc_p pc_g pc_b pc_e pc_a]> regs) r1 p0 g0 b0 e0 a0 storev
-    → std W C !! pc_a = Some ρ
+    → std W !! pc_a = Some ρ
     → mem0 !! a0 = Some oldv (*?*)
     -> ρ ≠ Revoked
     -> (∀ m, ρ ≠ Frozen m)
