theories/monotone.v
@@ -15,9 +15,7 @@ Section monotone.
 
   Notation STS := (leibnizO (STS_states * STS_rels)).
   Notation STS_STD := (leibnizO (STS_std_states Addr region_type)).
-  Notation CVIEW := (prodO STS_STD STS).
-  Notation WORLD := (gmapO CmptName CVIEW).
-  Implicit Types WC : CVIEW.
+  Notation WORLD := (prodO STS_STD STS).
   Implicit Types W : WORLD.
   Implicit Types C : CmptName.
 
@@ -26,96 +24,48 @@ Section monotone.
   Implicit Types w : (leibnizO Word).
   Implicit Types interp : (D).
 
-  Lemma region_state_pub_perm_cview WC WC' a :
-    related_sts_pub_cview WC WC'
-    → (std_cview WC) !! a = Some Permanent
-    -> (std_cview WC') !! a = Some Permanent.
+  Lemma region_state_pub_perm W W' a :
+    related_sts_pub_world W W'
+    → (std W) !! a = Some Permanent
+    -> (std W') !! a = Some Permanent.
   Proof.
     intros Hrelated Hstate.
     destruct Hrelated as [ [Hdom_sta Hrelated ] _]. simpl in *.
-    assert (is_Some ((std_cview WC') !! a)) as [y Hy].
+    assert (is_Some ((std W') !! a)) as [y Hy].
     { rewrite -elem_of_dom. apply elem_of_subseteq in Hdom_sta. apply Hdom_sta. rewrite elem_of_dom;eauto. }
     specialize (Hrelated a Permanent y Hstate Hy).
     apply std_rel_pub_rtc_Permanent in Hrelated; subst; auto.
   Qed.
 
-  Lemma region_state_pub_perm W W' C a :
-    related_sts_pub_world W W' C
-    → (std W C) !! a = Some Permanent
-    -> (std W' C) !! a = Some Permanent.
-  Proof.
-    rewrite /std.
-    intros Hrelated Hstate.
-    destruct (W !! C) as [WC|] eqn:HWC; last done.
-    destruct Hrelated as [Hdom_W Hrelated ].
-    assert (is_Some (W' !! C)) as [WC' HWC'].
-    { rewrite -elem_of_dom. apply elem_of_subseteq in Hdom_W.
-      apply Hdom_W. rewrite elem_of_dom;eauto. }
-    rewrite HWC'.
-    eapply region_state_pub_perm_cview; eauto.
-  Qed.
-
-  Lemma region_state_pub_temp_cview WC WC' a :
-    related_sts_pub_cview WC WC'
-    → (std_cview WC) !! a = Some Temporary
-    -> (std_cview WC') !! a = Some Temporary.
+  Lemma region_state_pub_temp W W' a :
+    related_sts_pub_world W W'
+    → (std W) !! a = Some Temporary
+    -> (std W') !! a = Some Temporary.
   Proof.
     intros Hrelated Hstate.
     destruct Hrelated as [ [Hdom_sta Hrelated ] _]. simpl in *.
-    assert (is_Some ((std_cview WC') !! a)) as [y Hy].
+    assert (is_Some ((std W') !! a)) as [y Hy].
     { rewrite -elem_of_dom. apply elem_of_subseteq in Hdom_sta. apply Hdom_sta. rewrite elem_of_dom;eauto. }
     specialize (Hrelated _ Temporary y Hstate Hy).
     apply std_rel_pub_rtc_Temporary in Hrelated; subst; auto.
   Qed.
 
-  Lemma region_state_pub_temp W W' C a :
-    related_sts_pub_world W W' C
-    → (std W C) !! a = Some Temporary
-    -> (std W' C) !! a = Some Temporary.
-  Proof.
-    rewrite /std.
-    intros Hrelated Hstate.
-    destruct (W !! C) as [WC|] eqn:HWC; last done.
-    destruct Hrelated as [Hdom_W Hrelated ].
-    assert (is_Some (W' !! C)) as [WC' HWC'].
-    { rewrite -elem_of_dom. apply elem_of_subseteq in Hdom_W.
-      apply Hdom_W. rewrite elem_of_dom;eauto. }
-    rewrite HWC'.
-    eapply region_state_pub_temp_cview; eauto.
-  Qed.
-
-  Lemma region_state_priv_perm_cview WC WC' a :
-    related_sts_priv_cview WC WC'
-    → (std_cview WC) !! a = Some Permanent
-    -> (std_cview WC') !! a = Some Permanent.
+  Lemma region_state_priv_perm W W' a :
+    related_sts_priv_world W W'
+    → (std W) !! a = Some Permanent
+    -> (std W') !! a = Some Permanent.
   Proof.
     intros Hrelated Hstate.
     destruct Hrelated as [ [Hdom_sta Hrelated ] _]. simpl in *.
-    assert (is_Some ((std_cview WC') !! a)) as [y Hy].
+    assert (is_Some ((std W') !! a)) as [y Hy].
     { rewrite -elem_of_dom. apply elem_of_subseteq in Hdom_sta. apply Hdom_sta. rewrite elem_of_dom;eauto. }
     specialize (Hrelated a Permanent y Hstate Hy).
     eapply std_rel_rtc_Permanent in Hrelated;subst;auto.
   Qed.
 
-  Lemma region_state_priv_perm W W' C a :
-    related_sts_priv_world W W' C
-    → (std W C) !! a = Some Permanent
-    -> (std W' C) !! a = Some Permanent.
-  Proof.
-    rewrite /std.
-    intros Hrelated Hstate.
-    destruct (W !! C) as [WC|] eqn:HWC; last done.
-    destruct Hrelated as [Hdom_W Hrelated ].
-    assert (is_Some (W' !! C)) as [WC' HWC'].
-    { rewrite -elem_of_dom. apply elem_of_subseteq in Hdom_W.
-      apply Hdom_W. rewrite elem_of_dom;eauto. }
-    rewrite HWC'.
-    eapply region_state_priv_perm_cview; eauto.
-  Qed.
-
-  Lemma region_state_nwl_monotone W W' C a l :
-    related_sts_pub_world W W' C →
-    region_state_nwl W C a l -> region_state_nwl W' C a l.
+  Lemma region_state_nwl_monotone W W' a l :
+    related_sts_pub_world W W' →
+    region_state_nwl W a l -> region_state_nwl W' a l.
   Proof.
     rewrite /region_state_nwl.
     intros  Hrelated Hstate; simplify_eq.
@@ -126,30 +76,30 @@ Section monotone.
       + eapply region_state_pub_temp in Hstate; eauto.
   Qed.
 
-  Lemma region_state_nwl_monotone_nl W W' C a :
-    related_sts_priv_world W W' C →
-    region_state_nwl W C a Global -> region_state_nwl W' C a Global.
+  Lemma region_state_nwl_monotone_nl W W' a :
+    related_sts_priv_world W W' →
+    region_state_nwl W a Global -> region_state_nwl W' a Global.
   Proof.
     rewrite /region_state_nwl.
     intros Hrelated Hstate; simplify_eq.
     eapply region_state_priv_perm;eauto.
   Qed.
 
-  Lemma region_state_pwl_monotone W W' C a :
-    related_sts_pub_world W W' C →
-    region_state_pwl W C a -> region_state_pwl W' C a.
+  Lemma region_state_pwl_monotone W W' a :
+    related_sts_pub_world W W' →
+    region_state_pwl W a -> region_state_pwl W' a.
   Proof.
     rewrite /region_state_pwl /region_state_nwl.
     intros Hrelated Hstate; simplify_eq.
     eapply region_state_pub_temp in Hstate; eauto.
   Qed.
 
-  Lemma region_state_nwl_future W W' C l l' p a:
+  Lemma region_state_nwl_future W W' l l' p a:
     LocalityFlowsTo l' l ->
     (if isWL p then l = Local else True) ->
-    (@future_world Σ _ l' W W' C) -∗
-    ⌜if isWL p then region_state_pwl W C a else region_state_nwl W C a l⌝ -∗
-    ⌜region_state_nwl W' C a l'⌝.
+    (@future_world Σ l' W W') -∗
+    ⌜if isWL p then region_state_pwl W a else region_state_nwl W a l⌝ -∗
+    ⌜region_state_nwl W' a l'⌝.
   Proof.
     intros Hlflows Hloc. iIntros "Hfuture %".
     rewrite /future_world.
@@ -161,17 +111,17 @@ Section monotone.
       + subst l.
         rewrite /region_state_nwl.
         right; eapply region_state_pub_temp; eauto.
-      + generalize (region_state_nwl_monotone _ _ _ _ _ Hf H).
+      + generalize (region_state_nwl_monotone _ _ _ _ Hf H).
         destruct l; auto.
   Qed.
 
-  Lemma region_state_future W W' C l l' p p' a:
+  Lemma region_state_future W W' l l' p p' a:
     PermFlowsTo p' p ->
     LocalityFlowsTo l' l ->
     (if isWL p then l = Local else True) ->
-    (@future_world Σ _ l' W W' C) -∗
-    ⌜if isWL p then region_state_pwl W C a else region_state_nwl W C a l⌝ -∗
-    ⌜if isWL p' then region_state_pwl W' C a else region_state_nwl W' C a l'⌝.
+    (@future_world Σ l' W W') -∗
+    ⌜if isWL p then region_state_pwl W a else region_state_nwl W a l⌝ -∗
+    ⌜if isWL p' then region_state_pwl W' a else region_state_nwl W' a l'⌝.
   Proof.
     intros Hpflows Hlflows Hloc. iIntros "Hfuture %Hstate".
     case_eq (isWL p'); intros Hpwlp'.
@@ -185,79 +135,62 @@ Section monotone.
     - iApply (region_state_nwl_future with "Hfuture"); eauto.
   Qed.
 
-  Lemma region_state_Revoked_monotone_cview (WC WC' : CVIEW) (a : Addr) :
-    related_sts_pub_cview WC WC' →
-    (std_cview WC) !! a = Some Revoked ->
-    (std_cview WC') !! a = Some Revoked ∨
-    (std_cview WC') !! a = Some Temporary ∨
-    (std_cview WC') !! a = Some Permanent.
+  Lemma region_state_Revoked_monotone (W W' : WORLD) (a : Addr) :
+    related_sts_pub_world W W' →
+    (std W) !! a = Some Revoked ->
+    (std W') !! a = Some Revoked ∨
+    (std W') !! a = Some Temporary ∨
+    (std W') !! a = Some Permanent.
   Proof.
-    rewrite /region_state_pwl /std_cview.
+    rewrite /region_state_pwl /std.
     intros Hrelated Hstate.
     destruct Hrelated as [ [Hdom_sta Hrelated ] _]. simpl in *.
-    assert (is_Some (WC'.1 !! a)) as [y Hy].
+    assert (is_Some (W'.1 !! a)) as [y Hy].
     { rewrite -elem_of_dom. apply elem_of_subseteq in Hdom_sta. apply Hdom_sta. rewrite elem_of_dom ;eauto. }
     specialize (Hrelated _ Revoked y Hstate Hy).
     apply std_rel_pub_rtc_Revoked in Hrelated; auto.
     destruct Hrelated as [Hperm | [Hmono | Hrev] ]; subst; auto.
   Qed.
 
-  Lemma region_state_Revoked_monotone (W W' : WORLD) (C : CmptName) (a : Addr) :
-    related_sts_pub_world W W' C →
-    (std W C) !! a = Some Revoked ->
-    (std W' C) !! a = Some Revoked ∨
-    (std W' C) !! a = Some Temporary ∨
-    (std W' C) !! a = Some Permanent.
-  Proof.
-    rewrite /region_state_pwl /std.
-    intros [Hdom_W Hrelated] Hstate.
-    destruct (W!!C) as [WC|] eqn:HWC; last done.
-    assert (is_Some (W' !! C)) as [WC' HWC'].
-    { rewrite -elem_of_dom. apply elem_of_subseteq in Hdom_W.
-      apply Hdom_W. rewrite elem_of_dom ;eauto. }
-    rewrite HWC'.
-    eapply region_state_Revoked_monotone_cview; eauto.
-  Qed.
-
   Lemma monoReq_mono_pub_nwl W W' C (P : D) a p g:
-    related_sts_pub_world W W' C
-    -> region_state_nwl W C a g
+    related_sts_pub_world W W'
+    -> region_state_nwl W a g
     -> monoReq W C a p P
     -∗ monoReq W' C a p P.
   Proof.
     intros Hrelated Hstate; simplify_eq.
     iIntros "HmonoW"; rewrite /monoReq.
     destruct g.
-    - pose proof (region_state_pub_perm _ _ _ _ Hrelated Hstate) as Hnext_state.
+    - pose proof (region_state_pub_perm _ _ _ Hrelated Hstate) as Hnext_state.
       by rewrite Hstate Hnext_state.
     - destruct Hstate as [Hstate|Hstate].
-      + pose proof (region_state_pub_perm _ _ _ _ Hrelated Hstate) as Hnext_state.
+      + pose proof (region_state_pub_perm _ _ _ Hrelated Hstate) as Hnext_state.
         by rewrite Hstate Hnext_state.
-      + pose proof (region_state_pub_temp _ _ _ _ Hrelated Hstate) as Hnext_state.
+      + pose proof (region_state_pub_temp _ _ _ Hrelated Hstate) as Hnext_state.
         by rewrite Hstate Hnext_state.
   Qed.
 
   Lemma monoReq_mono_pub_pwl W W' C (P : D) a p:
-    related_sts_pub_world W W' C
-    -> region_state_pwl W C a
+    related_sts_pub_world W W'
+    -> region_state_pwl W a
     -> monoReq W C a p P
     -∗ monoReq W' C a p P.
   Proof.
     intros Hrelated Hstate; simplify_eq.
     iIntros "HmonoW"; rewrite /monoReq.
-    pose proof (region_state_pub_temp _ _ _ _ Hrelated Hstate) as Hnext_state.
+    pose proof (region_state_pub_temp _ _ _ Hrelated Hstate) as Hnext_state.
     by rewrite Hstate Hnext_state.
   Qed.
 
   Lemma monoReq_mono_priv_nwl W W' C (P : D) a p:
-    related_sts_priv_world W W' C
-    -> region_state_nwl W C a Global
+    related_sts_priv_world W W'
+    -> region_state_nwl W a Global
     -> monoReq W C a p P
     -∗ monoReq W' C a p P.
   Proof.
     intros Hrelated Hstate; simplify_eq.
     iIntros "HmonoW"; rewrite /monoReq.
-    pose proof (region_state_priv_perm _ _ _ _ Hrelated Hstate) as Hnext_state.
+    pose proof (region_state_priv_perm _ _ _ Hrelated Hstate) as Hnext_state.
     by rewrite Hstate Hnext_state.
   Qed.
 
@@ -265,8 +198,8 @@ Section monotone.
     LocalityFlowsTo l' l
     -> PermFlowsTo p p'
     -> (if isWL p then l = Local else True)
-    -> (@future_world Σ _ l' W W' C)
-    -∗ ⌜if isWL p then region_state_pwl W C a else region_state_nwl W C a l⌝
+    -> (@future_world Σ l' W W')
+    -∗ ⌜if isWL p then region_state_pwl W a else region_state_nwl W a l⌝
     -∗ monoReq W C a p' P
     -∗ monoReq W' C a p' P.
   Proof.
@@ -284,7 +217,7 @@ Section monotone.
   Qed.
 
   Lemma interp_monotone_sd W W' C ot sb :
-    ⌜related_sts_priv_world W W' C⌝
+    ⌜related_sts_priv_world W W'⌝
     -∗ interp W C (WSealed ot sb) -∗ interp W' C (WSealed ot sb).
   Proof.
     iIntros (Hrelated) "#Hinterp".
@@ -302,7 +235,7 @@ Section monotone.
   Qed.
 
   Lemma interp_monotone W W' C w :
-    ⌜related_sts_pub_world W W' C⌝
+    ⌜related_sts_pub_world W W'⌝
     -∗ interp W C w -∗ interp W' C w.
   Proof.
     iIntros (Hrelated) "#Hw".
@@ -320,7 +253,7 @@ Section monotone.
       + iIntros "#Hrelated'".
         rewrite /future_world.
         iDestruct "Hrelated'" as "%Hrelated'".
-        iAssert (future_world Global W W'' C)%I as "Hrelated".
+        iAssert (future_world Global W W'')%I as "Hrelated".
         { rewrite /future_world.
           iPureIntro. apply related_sts_pub_priv_trans_world with W'; auto. }
         iSpecialize ("Hw" $! r W'' with "Hrelated").
@@ -328,7 +261,7 @@ Section monotone.
       + iIntros "#Hrelated'".
         rewrite /future_world.
         iDestruct "Hrelated'" as "%Hrelated'".
-        iAssert (future_world Local W W'' C)%I as "Hrelated".
+        iAssert (future_world Local W W'')%I as "Hrelated".
         { rewrite /future_world.
           iPureIntro. apply related_sts_pub_trans_world with W'; auto. }
         iSpecialize ("Hw" $! r W'' with "Hrelated").
@@ -389,7 +322,7 @@ Section monotone.
   Qed.
 
  Lemma interp_monotone_nl W W' C w :
-    ⌜related_sts_priv_world W W' C⌝
+    ⌜related_sts_priv_world W W'⌝
     -∗ ⌜isLocalWord w = false⌝
     -∗ interp W C w -∗ interp W' C w.
   Proof.
@@ -406,7 +339,7 @@ Section monotone.
       iIntros "#Hrelated'".
       rewrite /future_world.
       iDestruct "Hrelated'" as "%Hrelated'".
-      iAssert (future_world Global W W'' C)%I as "Hrelated".
+      iAssert (future_world Global W W'')%I as "Hrelated".
       { rewrite /future_world.
         iPureIntro. apply related_sts_priv_trans_world with W'; auto. }
       iSpecialize ("Hw" $! r W'' with "Hrelated").
@@ -481,7 +414,7 @@ Section monotone.
      pointer (p0, l, a2, a1, a0) ; simply a bundling of all individual monotonicity statements *)
 Lemma interp_monotone_generalW (W : WORLD) (C : CmptName) (ρ : region_type)
   (p p' p'' : Perm) (g g' : Locality) (b e a b' e' a' : Addr) :
-  std W C !! a' = Some ρ →
+  std W !! a' = Some ρ →
   withinBounds b' e' a' = true →
   PermFlowsTo p' p'' →
   canStore p' (WCap p g b e a) = true →
@@ -512,7 +445,7 @@ Qed.
 (* Analogous, but now we have the general monotonicity statement in case an integer z is written *)
 Lemma interp_monotone_generalZ (W : WORLD) (C : CmptName) (ρ : region_type)
   (p p' : Perm) (g : Locality) (b e a : Addr) z:
-  std W C !! a = Some ρ →
+  std W !! a = Some ρ →
   withinBounds b e a = true →
   PermFlowsTo p p' →
   interp W C (WCap p g b e a) -∗
@@ -531,7 +464,7 @@ Qed.
 Lemma interp_monotone_generalSr (W : WORLD) (C : CmptName) (ρ : region_type)
   (p p' : Perm) (g : Locality) (b e a : Addr)
   (sp : SealPerms) (sg : Locality) (sb se sa : OType) :
-  std W C !! a = Some ρ →
+  std W !! a = Some ρ →
   withinBounds b e a = true →
   PermFlowsTo p p' →
   interp W C (WCap p g b e a) -∗
@@ -549,7 +482,7 @@ Qed.
 Lemma interp_monotone_generalSd (W : WORLD) (C : CmptName) (ρ : region_type)
   (p p' : Perm) (g : Locality) (b e a : Addr)
   (ot : OType) (sb : Sealable) :
-  std W C !! a = Some ρ →
+  std W !! a = Some ρ →
   withinBounds b e a = true →
   PermFlowsTo p p' →
   interp W C (WCap p g b e a) -∗
